WIP: working on the separate compilation of Symbtablegen

x86/SymbtablegenSep.v
@@ -170,6 +170,144 @@ Lemma link_pres_wf_prog: forall p1 p2 p defs,
     wf_prog p.
 Admitted.
 
+
+(** ** Commutativity of linking and section generation *)
+
+Inductive list_in_order (A:Type) (f: A -> bool) : list A -> list A -> Prop :=
+| lorder_nil : list_in_order f nil nil
+| lorder_left_false : forall e l1 l2, 
+    f e = false -> list_in_order f l1 l2 -> list_in_order f (e :: l1) l2
+| lorder_right_false : forall e l1 l2,
+    f e = false -> list_in_order f l1 l2 -> list_in_order f l1 (e :: l2)
+| lorder_true : forall e l1 l2,
+    f e = true -> list_in_order f l1 l2 -> list_in_order f (e::l1) (e::l2).
+
+Lemma list_in_order_false_inv : forall (A:Type) (l1' l1 l2: list A) f e,
+    f e = false -> l1' = (e :: l1) -> list_in_order f l1' l2 -> list_in_order f l1 l2.
+Proof.
+  induction 3. 
+  - inv H0.
+  - inv H0. auto.
+  - apply lorder_right_false; auto.
+  - inv H0. congruence.
+Qed.
+
+Lemma list_in_order_true_inv : forall (A:Type) (l1' l1 l2: list A) f e,
+    f e = true -> l1' = (e :: l1) -> list_in_order f l1' l2 -> 
+    exists l3 l4, l2 = l3 ++ (e :: l4) /\ 
+             Forall (fun e' => f e' = false) l3 /\
+             list_in_order f l1 l4.
+Proof.
+  induction 3.
+  - inv H0.
+  - inv H0. congruence.
+  - subst. 
+    generalize (IHlist_in_order eq_refl).
+    destruct 1 as (l3 & l4 & EQ & FP & ORDER). subst.
+    exists (e0 :: l3), l4. split.
+    rewrite <- app_comm_cons. auto. split; auto.
+  - inv H0. exists nil, l2. split. auto.
+    split; auto.
+Qed.
+
+Lemma list_in_order_right_false_list : forall (A:Type) f (l2' l1 l2: list A),
+    Forall (fun e : A => f e = false) l2' ->
+    list_in_order f l1 l2 -> 
+    list_in_order f l1 (l2' ++ l2).
+Proof.
+  induction l2'.
+  - intros l1 l2 FALL ORDER. simpl. auto.
+  - intros l1 l2 FALL ORDER. simpl. 
+    generalize (Forall_inv FALL).
+    intros FLS.
+    apply lorder_right_false; auto.
+    apply IHl2'; auto.
+    rewrite Forall_forall in *.
+    intros. apply FALL. apply in_cons. auto.
+Qed.
+
+
+Lemma list_in_order_trans : forall (A:Type) f (l1 l2 l3: list A),
+    list_in_order f l1 l2 -> list_in_order f l2 l3 -> list_in_order f l1 l3.
+Proof.
+  intros A f l1 l2 l3 ORDER.
+  generalize l3.
+  induction ORDER.
+  - auto.
+  - intros l0 ORDER1. constructor; auto.
+  - intros l0 ORDER1. 
+    generalize (list_in_order_false_inv H (eq_refl (e::l2)) ORDER1). auto.
+  - intros l0 ORDER1.
+    generalize (list_in_order_true_inv H (eq_refl (e::l2)) ORDER1).
+    destruct 1 as (l2' & l2'' & EQ & FP & ORDER2).
+    subst.
+    apply IHORDER in ORDER2.
+    apply list_in_order_right_false_list; auto.
+    apply lorder_true; auto.
+Qed.    
+
+Lemma list_in_order_cons : forall (A:Type) f (l1 l2:list A) e,
+    list_in_order f l1 l2 -> list_in_order f (e::l1) (e::l2).
+Proof.
+  intros A f l1 l2 e ORDER.
+  destruct (f e) eqn:EQ.
+  apply lorder_true; auto.
+  apply lorder_left_false; auto.
+  apply lorder_right_false; auto.
+Qed.
+
+Lemma list_in_order_refl: forall (A:Type) f (l:list A),
+    list_in_order f l l.
+Proof.
+  induction l; intros.
+  - apply lorder_nil.
+  - apply list_in_order_cons. auto.
+Qed.
+
+
+Lemma partition_pres_list_in_order: forall (A:Type) pf f (l l1 l2: list A),
+    partition pf l = (l1, l2) ->
+    Forall (fun e => f e = false) l1 ->
+    list_in_order f l l2.
+Proof.
+  induction l.
+  - intros l1 l2 PART ALL. simpl in *. inv PART. constructor.
+  - intros l1 l2 PART ALL. simpl in *.
+    destruct (pf a).
+    + destruct (partition pf l) eqn:PART1. inv PART.
+      apply lorder_left_false. 
+      apply Forall_inv in ALL. auto.
+      apply IHl with l0; auto.
+      rewrite Forall_forall in *. intros. 
+      apply ALL; auto. apply in_cons. auto.
+    + destruct (partition pf l) eqn:PART1. inv PART.
+      apply list_in_order_cons. 
+      apply IHl with l1; auto.
+Qed.
+
+
+Lemma extern_var_init_data_nil : forall v,
+    is_var_internal v = false ->
+    get_def_init_data (Some (Gvar v)) = [].
+Proof.
+  intros v H. simpl in *. 
+  unfold is_var_internal in H. 
+  destruct (gvar_init v); try congruence.
+  destruct i; try congruence.
+  destruct l; try congruence.
+Qed.
+
+Lemma extern_init_data_nil : forall def,
+    is_def_internal is_fundef_internal def = false -> get_def_init_data def = nil.
+Proof.
+  intros def H.
+  destruct def. destruct g. 
+  - simpl in *. auto.
+  - simpl in H. apply extern_var_init_data_nil. auto.
+  - simpl in *. auto.
+Qed.
+
+
 Lemma acc_init_data_app : forall def l1 l2,
     (acc_init_data def l1) ++ l2 = acc_init_data def (l1 ++ l2).
 Proof.
@@ -187,10 +325,233 @@ Proof.
 Qed.
 
 
+Definition def_internal (iddef : ident * option (AST.globdef Asm.fundef unit)) :=
+  let '(_,def) := iddef in
+  is_def_internal is_fundef_internal def.
+
+Lemma acc_init_data_in_order_eq : forall defs1 defs2,
+    list_in_order def_internal defs1 defs2 ->
+    fold_right acc_init_data [] defs1 = fold_right acc_init_data [] defs2.
+Proof.
+  induction 1.
+  - simpl. auto.
+  - destruct e as (id, def). simpl.     
+    erewrite extern_init_data_nil; eauto.
+  - destruct e as (id, def). simpl.
+    erewrite extern_init_data_nil; eauto.
+  - destruct e as (id, def). simpl.
+    rewrite IHlist_in_order. auto.
+Qed.
+
+Lemma is_def_internal_dec' : forall (F V:Type) (f:F -> bool) (def: option (globdef F V)),
+    {is_def_internal f def = true} + {is_def_internal f def <> true}.
+Proof.
+  decide equality.
+Qed.
+
+Lemma is_def_internal_dec : forall (F V:Type) (f:F -> bool) (def: option (globdef F V)),
+    {is_def_internal f def = true} + {is_def_internal f def = false}.
+Proof.
+  intros F V f def.
+  generalize (is_def_internal_dec' f def).
+  intro H.
+  inv H. auto.
+  rewrite not_true_iff_false in H0. auto.
+Qed.
+
+
+Lemma link_fundef_inv1 : forall (F:Type) (f: AST.fundef F) f' e, 
+    link_fundef f (External e) = Some f' -> f = f'.
+Proof.
+  intros F f f' e LINK.
+  destruct f. simpl in *. destruct e; try congruence.
+  simpl in LINK. destruct (external_function_eq e0 e); congruence.
+Qed.
+
+Lemma link_extern_fundef_inv: forall (F:Type) 
+                                (f f' f'': AST.fundef F),
+    is_fundef_internal f = false ->
+    link f' f = Some f'' -> 
+    f' = f''.
+Proof.
+  intros F f f' f'' FINT LINK.
+  unfold link in LINK. 
+  Transparent Linker_fundef.
+  unfold Linker_fundef in LINK.
+  destruct f; simpl in *. congruence.
+  simpl in LINK.
+  apply link_fundef_inv1 in LINK. auto.
+Qed.
+
+Lemma link_extern_gfundef_inv: forall (F V:Type) (LV: Linker V)
+                             (f: AST.fundef F) (g g': (globdef (AST.fundef F) V)),
+    is_fundef_internal f = false ->
+    link g (Gfun f) = Some g' -> 
+    g = g'.
+Proof.
+  intros F V LV f g g' INT LINK.
+  destruct g. 
+  - unfold link in LINK. 
+    Transparent Linker_def.
+    unfold Linker_def in LINK.
+    simpl in LINK. destruct (link_fundef f0 f) eqn:LINKF; try congruence.
+    inv LINK.
+    generalize (link_extern_fundef_inv _ _ INT LINKF).
+    intros. subst.
+    auto.
+  - simpl in LINK. congruence.
+Qed.
+
+
+Lemma link_extern_var_inv: forall (V:Type) (LV:Linker V)
+                                (v v' v'': globvar V),
+    is_var_internal v = false ->
+    link v' v = Some v'' -> 
+    v' = v''.
+Proof.
+  intros V LV v v' v'' VINT LINK.
+  unfold link in LINK. 
+  Transparent Linker_vardef.
+  unfold Linker_vardef in LINK.
+  unfold link_vardef in LINK.
+  destruct (link (gvar_info v') (gvar_info v)) eqn:LINK_INFO; try congruence.
+  destruct (link (gvar_init v') (gvar_init v)) eqn:LINK_INIT; try congruence.
+  destruct (eqb (gvar_readonly v') (gvar_readonly v) && eqb (gvar_volatile v') (gvar_volatile v)) eqn:EQB; 
+    try congruence.
+  inv LINK.
+  destruct v; simpl in *. 
+  unfold link,link in LINK_INFO. 
+  
+  Admitted.
+
+Lemma link_extern_gvar_inv: forall (F V:Type) (LV: Linker V)
+                              (v: globvar V) (g g': (globdef (AST.fundef F) V)),
+    is_var_internal v = false ->
+    link g (Gvar v) = Some g' -> 
+    g = g'.
+Proof.
+  intros F V LV v g g' INT LINK.
+  destruct g. 
+  - unfold link in LINK. 
+    Transparent Linker_def.
+    unfold Linker_def in LINK.
+    simpl in LINK. congruence.
+  - simpl in LINK. 
+    destruct (link_vardef v0 v) eqn:LINKV; try congruence.
+    inv LINK.
+    generalize (link_extern_var_inv _ _ _ INT LINKV).
+    intros. subst.
+    auto.
+Qed.   
+
+
+Lemma link_def_inv2 : forall (F V: Type) (LV: Linker V) (def1 def2 def: option (globdef (AST.fundef F) V)),
+    def1 <> None ->
+    is_def_internal is_fundef_internal def2 = false ->
+    link_option def1 def2 = Some def ->
+    def = def1.
+Proof.
+  intros F V LV def1 def2 def NOTNONE INT LINK.
+  destruct def2. destruct g.
+  - simpl in *. unfold link_option in LINK.
+    destruct def1 as [|def1].
+    destruct (link g (Gfun f)) eqn:LEQ; try congruence.
+    inv LINK.
+    generalize (link_extern_gfundef_inv _ _ _ INT LEQ). intros. subst. auto.
+    inv LINK.
+    congruence.
+  - simpl in *. unfold link_option in LINK.
+    destruct def1 as [|def1].
+    destruct (link g (Gvar v)) eqn:LEQ; try congruence.
+    inv LINK.
+    generalize (link_extern_gvar_inv _ _ _ INT LEQ). intros. subst. auto.
+    congruence.    
+  - simpl in *. unfold link_option in LINK.
+    destruct def1 as [|def1].
+    inv LINK. auto.
+    inv LINK. auto.
+Qed.
+
+
+Lemma link_defs1_in_order : forall defs1 defs2 defs1_linked defs1_rest defs2_rest,
+    link_defs1 is_fundef_internal defs1 defs2 = Some (defs1_linked, defs1_rest, defs2_rest) ->
+    list_in_order def_internal defs1 defs1_linked /\
+    list_in_order def_internal defs2 defs2_rest.
+Proof.
+  induction defs1 as [|def1 defs1'].
+  - intros defs2 defs1_linked defs1_rest defs2_rest LINK.
+    simpl in *. inv LINK. split.
+    constructor.
+    apply list_in_order_refl.
+
+  - intros defs2 defs1_linked defs1_rest defs2_rest LINK.
+    simpl in LINK. destruct def1 as (id1, def1).
+    destruct (link_defs1 is_fundef_internal defs1' defs2) eqn:LINK1; try congruence.
+    destruct p as (p, defs2_rest').
+    destruct p as (defs1_linked', defs1_rest').
+    destruct (partition (fun '(id', _) => ident_eq id' id1) defs2_rest') as (defs2' & defs2_rest'') eqn:PART.
+    destruct defs2' as [| iddef2 defs2''].
+    + (** No definition with the same id found in defs2 *)
+      inv LINK.
+      generalize (IHdefs1' _ _ _ _ LINK1).
+      destruct 1 as (LORDER1 & LORDER2).
+      split; auto.      
+      apply list_in_order_cons; eauto.
+
+    + (** Some definition with the same id found in defs2 *)
+      destruct iddef2 as (id2 & def2).     
+      destruct (is_def_internal_dec is_fundef_internal def2) as [DEFINT2 | DEFINT2];
+        rewrite DEFINT2 in LINK.
+      destruct (is_def_internal_dec is_fundef_internal def1) as [DEFINT1 | DEFINT1];
+        rewrite DEFINT1 in LINK.
+      congruence.
+      inv LINK.
+      * (** The left definition is external and the right definition is internal.
+            The linking is delayed *)
+        generalize (IHdefs1' _ _ _ _ LINK1).
+        destruct 1 as (LORDER1 & LORDER2). split; auto.
+        apply lorder_left_false; auto.
+
+      * destruct (link_option def1 def2) as [def|] eqn:LINK_SYMB; inv LINK.
+        (** The right definition is external.
+            The linking proceeds normally *)
+        generalize (IHdefs1' _ _ _ _ LINK1).
+        destruct 1 as (LORDER1 & LORDER2).
+        assert (defs2'' = nil). admit.
+        subst. split.
+        ** destruct def1 as [def1|].
+           *** assert (Some def1 <> None) as NEQ by congruence .
+               generalize (link_def_inv2 _ def2 NEQ DEFINT2 LINK_SYMB).
+               intros. subst.
+               apply list_in_order_cons. auto.
+           *** simpl in LINK_SYMB. inv LINK_SYMB.
+               apply lorder_left_false; auto.
+               apply lorder_right_false; auto.
+        ** generalize (partition_pres_list_in_order _ def_internal _ PART).
+           intros LORDER3.
+           apply list_in_order_trans with defs2_rest'; auto.
+Admitted.          
+          
+                
 Lemma link_acc_init_data_comm : forall defs1 defs2 defs,
     link_defs is_fundef_internal defs1 defs2 = Some defs ->
-    fold_right acc_init_data [] defs = fold_right acc_init_data [] (defs1 ++ defs2).
-Admitted.
+    fold_right acc_init_data [] defs = 
+    fold_right acc_init_data [] defs1 ++ fold_right acc_init_data [] defs2.
+Proof.
+  intros defs1 defs2 defs LINK.
+  unfold link_defs in LINK.
+  destruct (link_defs1 is_fundef_internal defs1 defs2) eqn:LINK1; try inv LINK.
+  destruct p as (r & defs2_rest). destruct r as (defs1_linked & defs1_rest).
+  destruct (link_defs1 is_fundef_internal defs2_rest defs1_rest) eqn:LINK2; try inv H0.
+  destruct p. destruct p as (defs2_linked & p). inv H1.
+  rewrite fold_right_app. rewrite <- fold_right_acc_init_data_app.
+  apply link_defs1_in_order in LINK1. destruct LINK1 as (ORDER1 & ORDER2).
+  apply link_defs1_in_order in LINK2. destruct LINK2 as (ORDER3 & ORDER4).
+  generalize (list_in_order_trans ORDER2 ORDER3).
+  intros ORDER5.
+  rewrite (acc_init_data_in_order_eq ORDER1).
+  rewrite (acc_init_data_in_order_eq ORDER5). auto.
+Qed.
 
 
 Lemma acc_instrs_app : forall def l1 l2,
@@ -283,8 +644,8 @@ Proof.
   repeat f_equal.
   unfold create_sec_table. repeat f_equal.
   unfold create_data_section. f_equal.
-  rewrite fold_right_acc_init_data_app.
-  rewrite <- fold_right_app.
+  (* rewrite fold_right_acc_init_data_app. *)
+  (* rewrite <- fold_right_app. *)
   apply link_acc_init_data_comm; auto.
   unfold create_code_section. f_equal.
   rewrite fold_right_acc_instrs_app.
